doc(FirstOrder): Fix some typos and add a few docstrings (#878)

Foundation/FirstOrder/Basic/Syntax/Formula.lean
@@ -541,7 +541,7 @@ def lMap (Φ : L₁ →ᵥ L₂) {n} : Semiformula L₁ ξ n →ˡᶜ Semiformul
     (Semiformula.lMap Φ φ).freeVariables = φ.freeVariables := by
   induction φ using Semiformula.rec' <;> try simp [lMap_rel, lMap_nrel, freeVariables_rel, freeVariables_nrel, *]
 
-section enumarateFVar
+section enumerateFVar
 
 def fvarList {n : ℕ} : Semiformula L ξ n → List ξ
   |        ⊤ => []
@@ -555,18 +555,18 @@ def fvarList {n : ℕ} : Semiformula L ξ n → List ξ
 
 def idxOfFVar [DecidableEq ξ] (φ : Semiformula L ξ n) : ξ → ℕ := φ.fvarList.idxOf
 
-def enumarateFVar [Inhabited ξ] (φ : Semiformula L ξ n) : ℕ → ξ :=
+def enumerateFVar [Inhabited ξ] (φ : Semiformula L ξ n) : ℕ → ξ :=
   fun i ↦ if hi : i < φ.fvarList.length then φ.fvarList.get ⟨i, hi⟩ else default
 
-lemma enumarateFVar_idxOfFVar [DecidableEq ξ] [Inhabited ξ] {φ : Semiformula L ξ n} {x : ξ} (hx : x ∈ φ.fvarList) :
-    enumarateFVar φ (idxOfFVar φ x) = x := by
-  simpa [enumarateFVar, idxOfFVar]
+lemma enumerateFVar_idxOfFVar [DecidableEq ξ] [Inhabited ξ] {φ : Semiformula L ξ n} {x : ξ} (hx : x ∈ φ.fvarList) :
+    enumerateFVar φ (idxOfFVar φ x) = x := by
+  simpa [enumerateFVar, idxOfFVar]
   using fun h ↦ False.elim <| not_le.mpr (List.idxOf_lt_length_iff.mpr hx) h
 
 lemma mem_fvarList_iff_fvar? [DecidableEq ξ] {φ : Semiformula L ξ n} : x ∈ φ.fvarList ↔ φ.FVar? x := by
   induction φ using rec' <;> simp [fvarList, Semiterm.mem_fvarList_iff_fvar?, *]
 
-end enumarateFVar
+end enumerateFVar
 
 end Semiformula
 
